\color{blue}

**Solution**. FALSE.
$$
\begin{align}
\text{P}(X<-c) &=  \text{P}(\frac{X-\mu}{\sigma}<\frac{-c-\mu}{\sigma}) \\
&= \text{P}(Z<\frac{-c-\mu}{\sigma}), \hspace{1cm} \text{where } Z\sim\mathcal{N}(0,1) \\
&= \text{P}(Z<- \frac{c+\mu}{\sigma}) \\
&=  \text{P}(Z> \frac{c+\mu}{\sigma}), \hspace{1cm} \text{(by symmetry)}\\
&= 1- \text{P}(Z < \frac{c+\mu}{\sigma}) \\
&= 1- \text{P}(\frac{X-\mu}{\sigma} < \frac{c+\mu}{\sigma}) \\
&= 1- \text{P}(X-\mu < c+\mu) \\
&= 1- \text{P}(X< c+2\mu) 
\end{align}
$$
\color{black}

