\color{blue}

**Solution**.  
**(a)**  

$X-2Y+W$ is a normal variable, since linear combinations of normal variables are normal.  

- $\text{E}(X-2Y+W) = \text{E}(X) - 2\text{E}(Y) + \text{E}(W)  = 2-2+0 = 0$  
\vspace{6pt}
- $\text{Var}(\begin{bmatrix} X \\ Y \\ W \end{bmatrix})= \begin{bmatrix} \text{Var}(X) & \text{Cov}(X,Y) & \text{Cov}(X,W) \\ \text{Cov}(Y,X) & \text{Var}(Y)  & \text{Cov}(Y,W) \\ \text{Cov}(W,X) & \text{Cov}(W,Y) & \text{Var}(W) \end{bmatrix}$  
\vspace{6pt}
    - $\text{Cov}(X,Y) = \text{Cor}(X,Y)\sqrt{\text{Var}(X)\text{Var}(Y)} = -0.5\sqrt{2 2} = -1$  
    - $\text{Cov}(X,W) = \text{Cor}(X,W)\sqrt{\text{Var}(X)\text{Var}(W)} = 0\sqrt{2 2} = 0$  
    - $\text{Cov}(Y,W) = \text{Cor}(Y,W)\sqrt{\text{Var}(Y)\text{Var}(W)} = -0.5\sqrt{2 2} = -1$  
    
\vspace{10pt}

So, $\text{Var}(\begin{bmatrix} X \\ Y \\ W \end{bmatrix})  = \begin{bmatrix} 2& -1 & 0 \\ -1 &2&-1 \\ 0 & -1 & 2  \end{bmatrix}$  


Then, $X-2Y+W = \begin{bmatrix} 1 & -2 & 1 \end{bmatrix} \begin{bmatrix} X \\ Y \\ W \end{bmatrix} = \mathbb{A}\mathbf{X}, \hspace{0.2cm}\text{where }\mathbf{X} = \begin{bmatrix} X \\ Y \\ W \end{bmatrix}$  
$$
\begin{aligned}
\text{Var}(X-Y+W) = \text{Var}(\mathbb{A}\mathbf{X}) &= \mathbb{A}\text{Var}(\mathbf{X})\mathbb{A}^T \\
&= \begin{bmatrix} 1 & -2 & 1 \end{bmatrix} \begin{bmatrix} 2& -1 & 0 \\ -1 &2&-1 \\ 0 & -1 & 2  \end{bmatrix} \begin{bmatrix} 1 \\ -2 \\ 1 \end{bmatrix} \\
&= \begin{bmatrix} 1 & -2 & 1 \end{bmatrix} \begin{bmatrix} 2(1) + (-1)(-2) + 0(1) \\ (-1)1 + 2(-2) + (-1)1 \\ 0(1)+(-1)(-2)+2(1) \end{bmatrix} \\
&= \begin{bmatrix} 1 & -2 & 1 \end{bmatrix} \begin{bmatrix} 4 \\ -6 \\ 4 \end{bmatrix} \\
&= 1(4) + (-2)(-6) + 1(4) \\
&= 20
\end{aligned}
$$

\vspace{5pt} 
So, $\mathbf{X-Y+W\sim \mathcal{N}(0,20)}$  

\vspace{10pt} 
X+2W is a normal variable, since linear combinations of normal variables are normal. 

- $\text{E}(X+2W) = \text{E}(X)+ \text{E}(2W)  = 2+0 = 2$  
\vspace{6pt}
- $\text{Var}(X+2W)= \text{Var}(X) + \text{Var}(2W) = \text{Var}(X) + 2^2\text{Var}(W) = 2+4(2) = 10$  

So, $\mathbf{X+2W\sim \mathcal{N}(2,10)}$.

**(b)**
$\prob(Y<\frac{X+W+1}{2})= \prob(2Y<X+W+1) = \prob(-1<X+W-2Y) =$ `pnorm(-1,0,20,lower.tail=FALSE)`
\color{black}