
\color{blue}

**Solution**.  

**(a)**  $X-2Y+W$ is a normal variable, since linear combinations of multivariate normal variables are normal.  
We use linearity to find $\E(X-2Y+W)$.
\[
\E (X-2Y+W) = \E (X) - 2\E (Y) + \E (W)  = 2-2+0 = 0
\] 
There are different approaches to finding $\var(X-2Y+W)$. Here, we find the variance/covariance matrix of $\vec{U}=(X,Y,Z)$. First, we calculate the covariances.
\begin{eqnarray*}
\cov(X,Y) &=&  \cor(X,Y)\sqrt{\var(X)\, \var(Y)} = -0.5\sqrt{2\times 2} = -1
\\
\cov(X,W) &=& \cor(X,W)\sqrt{\var(X)\, \var(W)} = 0\sqrt{2\times 2} = 0
\\
\cov(Y,W) &=& \cor(Y,W)\sqrt{\var(Y)\, \var(W)} = -0.5\sqrt{2\times  2} = -1
\end{eqnarray*}
Then,
\[
\var\left(\vec{U})\right)
= 
\begin{bmatrix} \var(X) & \cov(X,Y) & \cov(X,W) \\ \cov(Y,X) & \var(Y)  & \cov(Y,W) \\ \cov(W,X) & \cov(W,Y) & \var(W) \end{bmatrix}
=  
\begin{bmatrix} 2& -1 & 0 \\ -1 &2&-1 \\ 0 & -1 & 2  \end{bmatrix}
\]
Then, we write $X-2Y+W$ in the form
\[
X-2Y+W = \begin{bmatrix} 1 & -2 & 1 \end{bmatrix} \begin{bmatrix} X \\ Y \\ W \end{bmatrix} = \mat{A}\vec{U}.
\]
We can now use the formula for the variance of a linear combination,
\begin{eqnarray*}
\var(X-Y+W) &=& \var(\mat{A}\vec{U}) = \mat{A}\var(\vec{U})\mat{A}^T \\
&=& \begin{bmatrix} 1 & -2 & 1 \end{bmatrix} \begin{bmatrix} 2& -1 & 0 \\ -1 &2&-1 \\ 0 & -1 & 2  \end{bmatrix} \begin{bmatrix} 1 \\ -2 \\ 1 \end{bmatrix} \\
&=& \begin{bmatrix} 1 & -2 & 1 \end{bmatrix} \begin{bmatrix} 2(1) + (-1)(-2) + 0(1) \\ (-1)1 + 2(-2) + (-1)1 \\ 0(1)+(-1)(-2)+2(1) \end{bmatrix} \\
&=& \begin{bmatrix} 1 & -2 & 1 \end{bmatrix} \begin{bmatrix} 4 \\ -6 \\ 4 \end{bmatrix} \\
&=& 1(4) + (-2)(-6) + 1(4) \\
&=& 20
\end{eqnarray*}
So, $X-Y+W\sim \normal(0,\sqrt{20})$.  

**(b)** We rewrite $\prob(2Y<X+W+1)$ as  $\prob(X+W-2Y>-1)$. From (a) this can be computed as

`1-pnorm(-1,mean=0,sd=sqrt(20))`

\color{black}

